tools/umpire/portableevaluation/testdata/normal/contract.pb
@@ -1,10 +1,10 @@
 
-Dworkflow-nexus.query.exact-action-caller-closure.evaluation-contract ©Akáİ­j;8¯ÓìE.‚š¼4?’SI#°,UßlS"ñ
+Dworkflow-nexus.query.exact-action-caller-closure.evaluation-contract s+ ‰êMÌÜÏ“oúÈnÈ†t‰\g'Âågn†"ñ
 umpire-experiment/v2Gsha256:dde2fb35891dcc0020dbedf301805feda1b5136ec8622dd67fdc47a3d00fb1a8Gsha256:d393ae60847c8524f3a57de6769478f95fd4a6a90a0fefcad6af118206d458af"Gsha256:f7a6ebefca8202c6a7c467fd516e54d162c7d1f254c6c9a1f004a7f0b4135ab8*ü
 umpire-runtime-configuration/v2Gsha256:21b4f7d0db2f68f939df901c2c5d146b1be3e45e55ad6cc171445fda5f29c1d5Gsha256:7c4c35a8031d07ff55ef5e83b90c64e63cbc6b196642c379ed75b5fc461f3a67"Gsha256:3b8bae9ef57fa5f400076af50d01a283d8b928481d654abd0d3c39dd72ea2f6c2€
 5workflow-nexus.query.exact-action-caller-closure.testGsha256:9d4a0056098a5c4202835fad9c502fbeeb59aba871e5dbc4947046583cbd9e77:{
-0workflow-nexus.query.exact-action-caller-closureGsha256:d393ae60847c8524f3a57de6769478f95fd4a6a90a0fefcad6af118206d458afB.€€@€€€€  @(N2
-42949672958€ê0@€€H€€€PÀ©J¤:
+0workflow-nexus.query.exact-action-caller-closureGsha256:d393ae60847c8524f3a57de6769478f95fd4a6a90a0fefcad6af118206d458afB1€€@€€€€  @(N2
+42949672958€ê0@€€H€€€PÀ©XNJ¤:
 }
 2temporal.nexus.observation-program.basic-lifecycleGsha256:1ab36fdcd2978dec901678491646ec67fe0fc1d3bd1883e599bc2c53810b34808
 &Temporal/System/Nexus/Observation.lean"
